.lake/build/ir/Stlc/open_close.c
@@ -178,58 +178,61 @@ x_13 = !lean_is_exclusive(x_3);
 if (x_13 == 0)
 {
 lean_object* x_14; lean_object* x_15; lean_object* x_16; lean_object* x_17; 
-x_14 = lean_ctor_get(x_3, 0);
+x_14 = lean_ctor_get(x_3, 1);
 x_15 = lean_unsigned_to_nat(1u);
 x_16 = lean_nat_add(x_1, x_15);
 x_17 = l_Trm_opening(x_16, x_2, x_14);
 lean_dec(x_16);
-lean_ctor_set(x_3, 0, x_17);
+lean_ctor_set(x_3, 1, x_17);
 return x_3;
 }
 else
 {
-lean_object* x_18; lean_object* x_19; lean_object* x_20; lean_object* x_21; lean_object* x_22; 
+lean_object* x_18; lean_object* x_19; lean_object* x_20; lean_object* x_21; lean_object* x_22; lean_object* x_23; 
 x_18 = lean_ctor_get(x_3, 0);
+x_19 = lean_ctor_get(x_3, 1);
+lean_inc(x_19);
 lean_inc(x_18);
 lean_dec(x_3);
-x_19 = lean_unsigned_to_nat(1u);
-x_20 = lean_nat_add(x_1, x_19);
-x_21 = l_Trm_opening(x_20, x_2, x_18);
-lean_dec(x_20);
-x_22 = lean_alloc_ctor(2, 1, 0);
-lean_ctor_set(x_22, 0, x_21);
-return x_22;
+x_20 = lean_unsigned_to_nat(1u);
+x_21 = lean_nat_add(x_1, x_20);
+x_22 = l_Trm_opening(x_21, x_2, x_19);
+lean_dec(x_21);
+x_23 = lean_alloc_ctor(2, 2, 0);
+lean_ctor_set(x_23, 0, x_18);
+lean_ctor_set(x_23, 1, x_22);
+return x_23;
 }
 }
 default: 
 {
-uint8_t x_23; 
-x_23 = !lean_is_exclusive(x_3);
-if (x_23 == 0)
+uint8_t x_24; 
+x_24 = !lean_is_exclusive(x_3);
+if (x_24 == 0)
 {
-lean_object* x_24; lean_object* x_25; lean_object* x_26; lean_object* x_27; 
-x_24 = lean_ctor_get(x_3, 0);
-x_25 = lean_ctor_get(x_3, 1);
-x_26 = l_Trm_opening(x_1, x_2, x_24);
+lean_object* x_25; lean_object* x_26; lean_object* x_27; lean_object* x_28; 
+x_25 = lean_ctor_get(x_3, 0);
+x_26 = lean_ctor_get(x_3, 1);
 x_27 = l_Trm_opening(x_1, x_2, x_25);
-lean_ctor_set(x_3, 1, x_27);
-lean_ctor_set(x_3, 0, x_26);
+x_28 = l_Trm_opening(x_1, x_2, x_26);
+lean_ctor_set(x_3, 1, x_28);
+lean_ctor_set(x_3, 0, x_27);
 return x_3;
 }
 else
 {
-lean_object* x_28; lean_object* x_29; lean_object* x_30; lean_object* x_31; lean_object* x_32; 
-x_28 = lean_ctor_get(x_3, 0);
-x_29 = lean_ctor_get(x_3, 1);
+lean_object* x_29; lean_object* x_30; lean_object* x_31; lean_object* x_32; lean_object* x_33; 
+x_29 = lean_ctor_get(x_3, 0);
+x_30 = lean_ctor_get(x_3, 1);
+lean_inc(x_30);
 lean_inc(x_29);
-lean_inc(x_28);
 lean_dec(x_3);
-x_30 = l_Trm_opening(x_1, x_2, x_28);
 x_31 = l_Trm_opening(x_1, x_2, x_29);
-x_32 = lean_alloc_ctor(3, 2, 0);
-lean_ctor_set(x_32, 0, x_30);
-lean_ctor_set(x_32, 1, x_31);
-return x_32;
+x_32 = l_Trm_opening(x_1, x_2, x_30);
+x_33 = lean_alloc_ctor(3, 2, 0);
+lean_ctor_set(x_33, 0, x_31);
+lean_ctor_set(x_33, 1, x_32);
+return x_33;
 }
 }
 }
@@ -275,29 +278,31 @@ return x_9;
 }
 case 2:
 {
-lean_object* x_10; lean_object* x_11; 
+lean_object* x_10; lean_object* x_11; lean_object* x_12; 
 lean_dec(x_5);
 lean_dec(x_3);
 lean_dec(x_2);
 x_10 = lean_ctor_get(x_1, 0);
 lean_inc(x_10);
+x_11 = lean_ctor_get(x_1, 1);
+lean_inc(x_11);
 lean_dec(x_1);
-x_11 = lean_apply_1(x_4, x_10);
-return x_11;
+x_12 = lean_apply_2(x_4, x_10, x_11);
+return x_12;
 }
 default: 
 {
-lean_object* x_12; lean_object* x_13; lean_object* x_14; 
+lean_object* x_13; lean_object* x_14; lean_object* x_15; 
 lean_dec(x_4);
 lean_dec(x_3);
 lean_dec(x_2);
-x_12 = lean_ctor_get(x_1, 0);
-lean_inc(x_12);
-x_13 = lean_ctor_get(x_1, 1);
+x_13 = lean_ctor_get(x_1, 0);
 lean_inc(x_13);
+x_14 = lean_ctor_get(x_1, 1);
+lean_inc(x_14);
 lean_dec(x_1);
-x_14 = lean_apply_2(x_5, x_12, x_13);
-return x_14;
+x_15 = lean_apply_2(x_5, x_13, x_14);
+return x_15;
 }
 }
 }
@@ -953,60 +958,63 @@ x_14 = !lean_is_exclusive(x_3);
 if (x_14 == 0)
 {
 lean_object* x_15; lean_object* x_16; lean_object* x_17; lean_object* x_18; 
-x_15 = lean_ctor_get(x_3, 0);
+x_15 = lean_ctor_get(x_3, 1);
 x_16 = lean_unsigned_to_nat(1u);
 x_17 = lean_nat_add(x_1, x_16);
 lean_dec(x_1);
 x_18 = l_Trm_closing(x_17, x_2, x_15);
-lean_ctor_set(x_3, 0, x_18);
+lean_ctor_set(x_3, 1, x_18);
 return x_3;
 }
 else
 {
-lean_object* x_19; lean_object* x_20; lean_object* x_21; lean_object* x_22; lean_object* x_23; 
+lean_object* x_19; lean_object* x_20; lean_object* x_21; lean_object* x_22; lean_object* x_23; lean_object* x_24; 
 x_19 = lean_ctor_get(x_3, 0);
+x_20 = lean_ctor_get(x_3, 1);
+lean_inc(x_20);
 lean_inc(x_19);
 lean_dec(x_3);
-x_20 = lean_unsigned_to_nat(1u);
-x_21 = lean_nat_add(x_1, x_20);
+x_21 = lean_unsigned_to_nat(1u);
+x_22 = lean_nat_add(x_1, x_21);
 lean_dec(x_1);
-x_22 = l_Trm_closing(x_21, x_2, x_19);
-x_23 = lean_alloc_ctor(2, 1, 0);
-lean_ctor_set(x_23, 0, x_22);
-return x_23;
+x_23 = l_Trm_closing(x_22, x_2, x_20);
+x_24 = lean_alloc_ctor(2, 2, 0);
+lean_ctor_set(x_24, 0, x_19);
+lean_ctor_set(x_24, 1, x_23);
+return x_24;
 }
 }
 default: 
 {
-uint8_t x_24; 
-x_24 = !lean_is_exclusive(x_3);
-if (x_24 == 0)
+uint8_t x_25; 
+x_25 = !lean_is_exclusive(x_3);
+if (x_25 == 0)
 {
-lean_object* x_25; lean_object* x_26; lean_object* x_27; lean_object* x_28; 
-x_25 = lean_ctor_get(x_3, 0);
-x_26 = lean_ctor_get(x_3, 1);
+lean_object* x_26; lean_object* x_27; lean_object* x_28; lean_object* x_29; 
+x_26 = lean_ctor_get(x_3, 0);
+x_27 = lean_ctor_get(x_3, 1);
 lean_inc(x_1);
-x_27 = l_Trm_closing(x_1, x_2, x_25);
 x_28 = l_Trm_closing(x_1, x_2, x_26);
-lean_ctor_set(x_3, 1, x_28);
-lean_ctor_set(x_3, 0, x_27);
+x_29 = l_Trm_closing(x_1, x_2, x_27);
+lean_ctor_set(x_3, 1, x_29);
+lean_ctor_set(x_3, 0, x_28);
 return x_3;
 }
 else
 {
-lean_object* x_29; lean_object* x_30; lean_object* x_31; lean_object* x_32; lean_object* x_33; 
-x_29 = lean_ctor_get(x_3, 0);
-x_30 = lean_ctor_get(x_3, 1);
+lean_object* x_30; lean_object* x_31; lean_object* x_32; lean_object* x_33; lean_object* x_34; 
+x_30 = lean_ctor_get(x_3, 0);
+x_31 = lean_ctor_get(x_3, 1);
+lean_inc(x_31);
 lean_inc(x_30);
-lean_inc(x_29);
 lean_dec(x_3);
 lean_inc(x_1);
-x_31 = l_Trm_closing(x_1, x_2, x_29);
 x_32 = l_Trm_closing(x_1, x_2, x_30);
-x_33 = lean_alloc_ctor(3, 2, 0);
-lean_ctor_set(x_33, 0, x_31);
-lean_ctor_set(x_33, 1, x_32);
-return x_33;
+x_33 = l_Trm_closing(x_1, x_2, x_31);
+x_34 = lean_alloc_ctor(3, 2, 0);
+lean_ctor_set(x_34, 0, x_32);
+lean_ctor_set(x_34, 1, x_33);
+return x_34;
 }
 }
 }
