Stlc/decidable.lean
@@ -1,0 +1,132 @@
+import Stlc.normalization
+
+open Typ
+open Trm
+open List
+open typing
+open valid_ctx
+open lc
+
+theorem typing_uniq :
+    ∀ t, lc t → ∀ Γ T1 T2,
+    typing Γ t T1 → typing Γ t T2 → T1 = T2 := by
+  intro t lct
+  induction lct
+  case lc_var x =>
+    intro Γ T1 T2 ty1 ty2
+    cases ty1
+    next _ bnd =>
+      cases ty2
+      next _ bnd' =>
+        simp [binds] at bnd bnd'
+        rw [bnd] at bnd'
+        simp at bnd'
+        exact bnd'
+  case lc_abs u T L a ih =>
+    intro Γ T1 T2 ty1 ty2
+    cases ty1
+    next L1 U1 h1 =>
+      cases ty2
+      next L2 U2 h2 =>
+        have ⟨x,hx⟩ := pick_fresh u (L ∪ L1 ∪ L2)
+        simp at hx ⊢
+        apply ih x hx.1 ((x,T) :: Γ) U1 U2 (h1 x hx.2.1) (h2 x hx.2.2.1)
+  case lc_app t1 t2 lct1 lct2 ih1 ih2 =>
+    intro Γ T1 T2 ty1 ty2
+    cases ty1
+    next S1 sy1 sy2 =>
+      cases ty2
+      next U1 uy1 uy2 =>
+        have this := ih1 _ _ _ sy2 uy2
+        have this2 := ih2 _ _ _ sy1 uy1
+        simp [this2] at this
+        exact this
+
+theorem typing_decidable :
+    ∀ t Γ, lc t → valid_ctx Γ →
+    (∃ T, typing Γ t T) ∨ ¬ (∃ T, typing Γ t T) := by
+  intro t Γ lct vld
+  induction lct generalizing Γ
+  case lc_var x =>
+    match h : (get x Γ) with
+    | some T =>
+        left
+        use T
+        apply typ_var Γ x T vld h
+    | none =>
+        right
+        rintro ⟨T, typ⟩
+        cases typ
+        next _ ih =>
+          simp [h] at ih
+  case lc_abs u T L a ih =>
+    have ⟨x,hx⟩ := pick_fresh u (L ∪ context_terms Γ)
+    simp at hx
+    cases H : (ih x hx.1 ((x,T) :: Γ)
+        (valid_push Γ x T vld (not_context_terms_to_not_in_context _ _ hx.2.1)))
+    next pos =>
+      rcases pos with ⟨S, p⟩
+      left
+      use (T -> S)
+      apply (typ_abs (fv u ∪ context_terms Γ) Γ)
+      intro y hy
+      simp at hy
+      apply typing_rename _ _ _ _ _ _
+              hx.2.2 (not_context_terms_to_not_in_context _ _ hx.2.1)
+              hy.1 ((not_context_terms_to_not_in_context _ _ hy.2)) p
+    next neg =>
+      right
+      rintro ⟨S,p⟩
+      cases p
+      next L' S' h =>
+        have ⟨z,hz⟩ := pick_fresh u (L' ∪ context_terms Γ)
+        simp at hz
+        apply neg
+        use S'
+        apply typing_rename _ _ _ _ _ _
+                hz.2.2 ((not_context_terms_to_not_in_context _ _ hz.2.1))
+                hx.2.2 ((not_context_terms_to_not_in_context _ _ hx.2.1)) (h z hz.1)
+  case lc_app t1 t2 lc1 lc2 ih1 ih2 =>
+    have this := ih1 Γ vld
+    have this2 := ih2 Γ vld
+    cases this
+    next pos =>
+      rcases pos with ⟨T,p1⟩
+      cases this2
+      next pos2 =>
+        rcases pos2 with ⟨S,p2⟩
+        match T with
+        | typ_base =>
+          right
+          rintro ⟨T, P⟩
+          cases P
+          next S ty1 ty2 =>
+            have q:= typing_uniq _ lc1 _ _ _ p1 ty2
+            simp at q
+        | typ_arrow S1 S2 =>
+          by_cases h : S1 = S
+          . left
+            use S2
+            rw [← h] at p2
+            apply typ_app Γ t1 t2 S1 S2 p1 p2
+          . right
+            rintro ⟨U, P⟩
+            cases P
+            next V ty1 ty2 =>
+              have q := typing_uniq _ lc1 _ _ _ p1 ty2
+              simp at q
+              have q' := typing_uniq _ lc2 _ _ _ p2 ty1
+              rw [← q'] at q
+              apply (h q.1)
+      next neg2 =>
+        right
+        rintro ⟨T, P⟩
+        cases P
+        next T1 ty1 ty2 =>
+          apply neg2 ⟨_ , ty1⟩
+    next neg =>
+      right
+      rintro ⟨T, P⟩
+      cases P
+      next T1 ty1 ty2 =>
+        apply neg ⟨_ , ty2⟩
